Case_Study/Mode_Switch.thy
@@ -92,13 +92,20 @@ lemma kernel_mappings_heap_eq:
 interpretation kernel_mappings: heap_only global_mappings_of_all_processes
   by unfold_locales (rule kernel_mappings_heap_eq)
 
+(*
 lemma ptable_comp_asid:
   "\<lbrakk> (a, v) \<in> ptable_comp b hp hp' rt rt'; a \<noteq> b \<rbrakk> \<Longrightarrow> False"
   by (auto simp: ptable_comp_def)
+*)
+
+
 
 lemma asids_consistentD:
-  "\<lbrakk> asids_consistent {} s; root_map s (Addr r) = Some a \<rbrakk> \<Longrightarrow> (a, v) \<notin> incon_set s"
-  by (clarsimp simp: asids_consistent_def ran_def) blast
+  "\<lbrakk> asids_consistent {} s; root_map s (Addr r) = Some a ; Addr r \<in> set (root_log s) ; a \<noteq> asid s \<rbrakk> \<Longrightarrow>
+              (ptable_snapshot s) a v \<noteq> Incon \<and> ((ptable_snapshot s) a v = Miss \<or> 
+                                 (ptable_snapshot s) a v = Hit (pt_walk a (heap s) (Addr r) v) )"
+  by (clarsimp simp: asids_consistent_def ran_def) 
+  
 
 (*
 lemma kernel_data_asid_consistent_eq:
@@ -115,8 +122,7 @@ interpretation asids_consistent: heap_only "asids_consistent {}"
 lemma pde_comp_def_x:
  "ptable_comp a hp hp' rt rt' =
   (let walk = pt_walk a hp rt; walk' = pt_walk a hp' rt'
-  in {a} \<times>
-     {va. \<not>is_fault (walk va) \<and> \<not> is_fault (walk' va) \<and> walk va \<noteq> walk' va \<or> 
+  in  {va. \<not>is_fault (walk va) \<and> \<not> is_fault (walk' va) \<and> walk va \<noteq> walk' va \<or> 
           \<not>is_fault (walk va) \<and> is_fault (walk' va)})"
  by (auto simp add: ptable_comp_def Let_def)
 
@@ -126,8 +132,7 @@ lemma pde_comp_def_x:
 lemma pde_comp_def:
  "ptable_comp a hp hp' rt rt' \<equiv>
   let walk = pt_walk a hp rt; walk' = pt_walk a hp' rt'
-  in {a} \<times>
-     {va. \<not>is_fault (walk va) \<and> \<not> is_fault (walk' va) \<and> walk va \<noteq> walk' va \<or> 
+  in  {va. \<not>is_fault (walk va) \<and> \<not> is_fault (walk' va) \<and> walk va \<noteq> walk' va \<or> 
           \<not>is_fault (walk va) \<and> is_fault (walk' va)}"
  by (simp add: pde_comp_def_x)
 
@@ -135,17 +140,10 @@ lemma pde_comp_def:
 definition
   \<I>\<C> :: "p_state \<Rightarrow> 32 word set"
 where
-  "\<I>\<C> s \<equiv>  {vp. (asid s, Addr vp) \<in> incon_set s}" 
+  "\<I>\<C> s \<equiv>  {vp. Addr vp \<in> incon_set s}" 
 
 
-
-(* have new conditions for tlb_snapshot *)
-
-
-(* it is a lookup type, which means that we have to assume that from tlb_rel that, 
-  in the start, the tlb_snanpshot will be miss, no incon and no hit, so lets assume that  *)
-
-
+(*
 definition
   "snap_not_incon S s \<equiv> \<forall>a\<in>(ran (root_map s) - S). \<forall>v. ptable_snapshot s a v \<noteq> Incon"
 
@@ -153,6 +151,7 @@ definition
 
 definition
   "snap_miss_or_consistent_hit snp a mem rt \<equiv> \<forall>v. snp a v = Miss \<or> snp a v = Hit (pt_walk a mem rt v)"
+*)
 
 
 (* context switch code from sel4
@@ -178,26 +177,22 @@ definition
 
 *)
 
-definition "snp_incon_constraint S s \<equiv> {(a,v). a\<in>(ran (root_map s) - S) \<and> ptable_snapshot s a v = Incon }  \<subseteq>  incon_set s"
-
 (* we assume that the flush has happened after write to the page table *)
 
-lemma
-  "\<lbrakk>snp_incon_constraint S s ; asids_consistent {} s \<rbrakk>  \<Longrightarrow> snap_not_incon S s"
-  apply (clarsimp simp: snp_incon_constraint_def ptable_snapshot_def asids_consistent_def ran_def snap_not_incon_def)
-  by blast
-
-
+(*
 lemma asids_diff_incon_load_empty:
   "a \<noteq> a' \<Longrightarrow>  {a} \<times> UNIV \<inter> incon_load snp a' m rt = {}"
   apply (clarsimp simp: incon_load_def) 
   by blast
+*)
 
-
+(*
 lemma asids_diff_ptable_comp_empty:
   "a \<noteq> a' \<Longrightarrow>  {a} \<times> UNIV \<inter> ptable_comp a' h h' r r' = {}"
   apply (clarsimp simp: ptable_comp_def) 
   by blast
+
+
 
 
 lemma  asids_diff_snap_update_current_incon_load_same [simp]:
@@ -208,32 +203,41 @@ lemma  asids_diff_snap_update_current_incon_load_same [simp]:
 lemma asids_diff_snap_update_new_incon_load_same [simp]:
   "a \<noteq> a' \<Longrightarrow>  incon_load (snapshot_update_new' snp iset m_to_h h_to_h hp ttbr0 a') a m rt = incon_load snp a m rt"
   by (clarsimp simp: incon_load_def snapshot_update_new'_def) 
+ *)
+
 
 lemma asid_con_mode_upd:
   "asids_consistent S (mode_update upd s) = asids_consistent S s"
   by (clarsimp simp: asids_consistent_def)
 
-
+(*
 lemma asid_con_root_upd:
   "asids_consistent S (root_update upd s) = asids_consistent S s"
   by (clarsimp simp: asids_consistent_def)
+*)
 
+(*
 lemma asid_con_asid_upd:
   "asids_consistent S (asid_update upd s) = asids_consistent S s"
   by (clarsimp simp: asids_consistent_def)
+*)
 
+(*
 lemma asid_con_upd [simp]:
   "asids_consistent S (s\<lparr>root := r, asid := a, incon_set := is, ptable_snapshot := snp,   mode := m\<rparr>) = 
                  asids_consistent S (s\<lparr> incon_set := is\<rparr>)"
   by (clarsimp simp: asids_consistent_def)
+*)
 
+(*
 lemma not_range_asid_con_simp [simp]:
   "  0 \<notin> ran (root_map s)
          \<Longrightarrow> asids_consistent {} (s\<lparr>incon_set := incon_set s \<union> incon_load (ptable_snapshot s) 0 (heap s) (root s) \<union> ptable_comp 0 (heap s) (heap s) (root s) (Addr r) \<union> incon_load (ptable_snapshot s) a (heap s) (Addr r) \<rparr>) = 
       asids_consistent {} (s\<lparr>incon_set := incon_set s \<union> incon_load (ptable_snapshot s) a (heap s) (Addr r) \<rparr>)"
   apply (clarsimp simp: asids_consistent_def incon_load_def ran_def ptable_comp_def) by blast
+*)
 
-
+(*
 lemma not_range_asid_con_simp' [simp]:
   "  0 \<notin> ran (root_map s)
          \<Longrightarrow> asids_consistent {}
@@ -242,13 +246,138 @@ lemma not_range_asid_con_simp' [simp]:
      asids_consistent {}
               (s\<lparr>incon_set := incon_set s \<union> incon_load (snapshot_update_current' (ptable_snapshot s) ({asid s} \<times> UNIV \<inter> incon_set s) (heap s) (Addr r) (asid s)) (asid s) (heap s) (Addr r)\<rparr>)"
   apply (clarsimp simp: asids_consistent_def incon_load_def ran_def ptable_comp_def) by blast
+*)
 
+
+lemma [simp]:
+  "asid s \<noteq> 0 \<Longrightarrow>
+  incon_load_incon (snapshot_update_current'2 (ptable_snapshot s) (incon_set s) (heap s) (root s) (asid s)) 0 (heap s)  = 
+   incon_load_incon (ptable_snapshot s) 0 (heap s) "
+  by (clarsimp simp: incon_load_incon_def snapshot_update_current'2_def snapshot_update_current2_def)
+
+lemma  [simp]:
+  " asid s \<noteq> 0 \<Longrightarrow> 
+     incon_load2 (snapshot_update_current'2 (ptable_snapshot s) (incon_set s) (heap s) (root s) (asid s)) 0 (heap s) (root s) =
+     incon_load2 (ptable_snapshot s)  0 (heap s) (root s)"
+  by (clarsimp simp: incon_load2_def snapshot_update_current'2_def)
+
+lemma [simp]:
+  "0 \<noteq> a \<Longrightarrow> incon_load_incon
+                      (snapshot_update_current'2
+                        (snapshot_update_current'2 (ptable_snapshot s) (incon_set s) (heap s) (root s) (asid s))
+                        iset'
+                        (heap s) (Addr r) 0)
+                      a (heap s)   = 
+    incon_load_incon
+                      (snapshot_update_current'2 (ptable_snapshot s) (incon_set s) (heap s) (root s) (asid s))
+                      a (heap s) "
+  by (clarsimp simp: incon_load_incon_def snapshot_update_current'2_def snapshot_update_current2_def)
+
+
+lemma  [simp]:
+  " a \<noteq> asid s \<Longrightarrow> incon_load_incon (snapshot_update_current'2 (ptable_snapshot s) (incon_set s) (heap s) (root s) (asid s)) 
+                        a
+                      (heap s) 
+                        = 
+     incon_load_incon (ptable_snapshot s) 
+                        a
+                      (heap s) 
+                       "
+  by (clarsimp simp: incon_load_incon_def snapshot_update_current'2_def snapshot_update_current2_def)
+
+lemma [simp]:
+  "a \<noteq> asid s \<and> a \<noteq> 0 \<Longrightarrow> 
+    incon_load2
+                      (snapshot_update_current'2 (snapshot_update_current'2 (ptable_snapshot s) (incon_set s) (heap s) (root s) (asid s))
+                        iset'
+                        (heap s) (Addr r) 0)
+                      a (heap s) (Addr r) = 
+   incon_load2
+                     (ptable_snapshot s)
+                      a (heap s) (Addr r)"
+  by (clarsimp simp: incon_load2_def snapshot_update_current'2_def snapshot_update_current2_def) 
+
+lemma asid_rewrite:
+  "\<lbrakk>asids_consistent {} 
+     (s\<lparr>root := Addr r, asid := a, incon_set := {},
+                   ptable_snapshot := pt,
+                   mode := User\<rparr>);  0 \<notin> ran (root_map s) ; 0 \<noteq> asid s\<rbrakk>  \<Longrightarrow> 
+    asids_consistent {} 
+      (s\<lparr>root := Addr r, asid := a, incon_set := {},
+                   ptable_snapshot :=
+                     snapshot_update_current'2
+                      pt
+                     is'
+                      (heap s) (Addr r) 0,
+                   mode := User\<rparr>)"
+  apply (clarsimp simp: asids_consistent_def)
+  apply (rule conjI)
+   apply (clarsimp simp: snapshot_update_current'2_def snapshot_update_current2_def)
+   apply (rule conjI)
+    apply (clarsimp simp: ran_def)
+   apply (clarsimp simp: ran_def)
+
+  apply (subgoal_tac "aa \<noteq> 0")
+   apply (subgoal_tac "snapshot_update_current'2 pt is' (heap s) (Addr r) 0 aa v =
+                         pt aa v  ")
+    apply (simp only:)
+    apply (drule_tac x = ra in spec)
+    apply (drule_tac x = aa in spec)
+    apply clarsimp
+    apply (clarsimp simp: snapshot_update_current'2_def snapshot_update_current2_def)
+  by  (clarsimp simp: ran_def)
+
+lemma asid_rewrite2:
+  "\<lbrakk>asids_consistent {} 
+     (s\<lparr> incon_set := {},
+                   ptable_snapshot := pt,
+                   mode := User\<rparr>);  0 \<notin> ran (root_map s) ; 0 \<noteq> asid s\<rbrakk>  \<Longrightarrow> 
+    asids_consistent {} 
+      (s\<lparr> incon_set := {},
+                   ptable_snapshot :=
+                     snapshot_update_current'2
+                      pt
+                     is'
+                      (heap s) (root s) 0,
+                   mode := User\<rparr>)"
+  apply (clarsimp simp: asids_consistent_def)
+  apply (rule conjI)
+   apply (clarsimp simp: snapshot_update_current'2_def snapshot_update_current2_def)
+   apply (rule conjI ; clarsimp simp: ran_def)
+
+
+
+  apply clarsimp
+  apply (clarsimp simp: snapshot_update_current'2_def snapshot_update_current2_def)
+  apply (rule conjI)
+   apply (clarsimp simp: ran_def)
+   apply (rule conjI)
+    apply (clarsimp simp: ran_def)
+   apply (clarsimp simp: ran_def)
+   apply (drule_tac x = r in spec)
+   apply (drule_tac x = a in spec)
+   apply clarsimp
+   apply (drule_tac x = v in spec, simp)
+  apply clarsimp
+  apply (rule conjI)
+   apply clarsimp
+   apply (rule conjI)
+    apply (clarsimp simp: ran_def)
+   apply clarsimp
+   apply (drule_tac x = r in spec)
+   apply (drule_tac x = a in spec)
+   apply clarsimp
+   apply (drule_tac x = v in spec, simp)
+  apply clarsimp
+  apply (drule_tac x = r in spec)
+  apply (drule_tac x = a in spec)
+  apply clarsimp
+  by (drule_tac x = v in spec, simp)
 
 
 lemma new_context_switch:
-  "\<Turnstile> \<lbrace> \<lambda>s. mmu_layout s \<and> asids_consistent {} s (* all assigned asids are consistent *) \<and> mode s = Kernel \<and> snp_incon_constraint {} s \<and>  
-           snap_miss_or_consistent_hit (ptable_snapshot s) a (heap s) (Addr r)  (*new asid and the root are consistent or miss in the ptable snapshot *)\<and> 
-            0 \<notin> ran (root_map s)  (* reserved asid is not assigned *)\<and> root_map s (Addr r) = Some a \<and> Addr r \<in> set (root_log s)\<rbrace>
+  "\<Turnstile> \<lbrace> \<lambda>s. mmu_layout s \<and> asids_consistent {} s \<and> mode s = Kernel \<and>  \<I>\<C> s = {} \<and>
+            0 \<notin> ran (root_map s)  \<and> root_map s (Addr r) = Some a \<and> Addr r \<in> set (root_log s)\<rbrace>
             UpdateASID 0 ;; UpdateTTBR0 (Const r) ;; UpdateASID a ;; SetMode User
       \<lbrace>\<lambda>s. mmu_layout s \<and> \<I>\<C> s = {} \<and> mode s = User \<and> asids_consistent {} s \<rbrace>"
   apply vcgm
@@ -260,37 +389,154 @@ lemma new_context_switch:
   apply (rule conjI)
    apply (clarsimp simp: \<I>\<C>_def)
    apply (rule conjI)
-    apply (clarsimp simp: asids_consistentD)
+    apply (clarsimp simp: incon_load_incon_def snapshot_update_current'2_def snapshot_update_current2_def)
+    apply (rule conjI)
+     apply clarsimp
+     apply (clarsimp simp: asids_consistent_def)
+    apply (clarsimp simp: asids_consistent_def)
+   apply (clarsimp simp: incon_load2_def snapshot_update_current'2_def snapshot_update_current2_def split: if_split_asm)
    apply (rule conjI)
-    using asids_diff_incon_load_empty apply blast
-   apply (rule conjI)
-    using asids_diff_ptable_comp_empty apply blast
-   apply (case_tac "a \<noteq> asid s")
-    apply simp
-    apply (clarsimp simp: snap_miss_or_consistent_hit_def incon_load_def) 
-    apply (drule_tac x = "Addr x" in spec , erule disjE ; clarsimp)
+    apply clarsimp
+    apply (rule conjI)
+     apply (clarsimp simp:)
+     apply (subgoal_tac "Addr r = root s")
+      apply clarsimp
+     apply (clarsimp simp: mmu_layout_def)
+     apply (clarsimp simp: ran_def partial_inj_def)
+     apply force
+    apply (clarsimp simp:)
+    apply (clarsimp simp: asids_consistent_def)
+    apply (drule_tac x = "Addr r" in spec)
+    apply (drule_tac x = a in spec)
+    apply clarsimp
+    apply (drule_tac x = "Addr x" in spec)
+    apply (erule conjE)
+    apply (erule disjE)
+     apply clarsimp
+    apply clarsimp
+   apply (clarsimp simp:) 
+   apply (clarsimp simp: asids_consistent_def)
+   apply (drule_tac x = "Addr r" in spec)
+   apply (drule_tac x = a in spec)
    apply clarsimp
-   apply (case_tac "root s = Addr r")
-    apply (clarsimp simp: incon_load_def snapshot_update_current'_def snapshot_update_current_def split: if_split_asm)
-   apply (clarsimp simp: mmu_layout_def partial_inj_def) 
-   apply force
-  apply (subgoal_tac " asid s \<noteq> 0") 
-   prefer 2 
+   apply (drule_tac x = "Addr x" in spec)
+   apply (erule conjE)
+   apply (erule disjE)
+    apply clarsimp
+   apply clarsimp
+  apply (subgoal_tac "asid s \<noteq> 0 ")
+   prefer 2
    apply (clarsimp simp: mmu_layout_def ran_def)
   apply clarsimp
   apply (case_tac "a \<noteq> asid s")
-   apply simp
-   apply (subgoal_tac "incon_load (ptable_snapshot s) a (heap s) (Addr r) = {}")
-    apply (clarsimp simp: )
-   apply (clarsimp simp: snap_miss_or_consistent_hit_def incon_load_def) 
-   apply (drule_tac x = x in spec , erule disjE ; clarsimp)
-  apply (case_tac "root s = Addr r")
    apply clarsimp
-   apply (clarsimp simp: incon_load_def snapshot_update_current'_def snapshot_update_current_def split: if_split_asm)
-  apply (clarsimp simp: mmu_layout_def partial_inj_def) 
-  by force
+   apply (subgoal_tac "incon_load_incon (ptable_snapshot s) a (heap s)  = {}")
+    prefer 2
+    apply (clarsimp simp: incon_load_incon_def asids_consistent_def)
+   apply clarsimp
+   apply (subgoal_tac "incon_load2 (ptable_snapshot s) a (heap s) (Addr r) = {}")
+    prefer 2
+    apply (clarsimp simp: incon_load2_def asids_consistent_def)
+    apply (drule_tac x = "Addr r" in spec)
+    apply (drule_tac x = a in spec , simp)
+    apply (drule_tac x = x in spec)
+    apply force
+   apply clarsimp
+   apply (rule asid_rewrite)
+     prefer 2
+     apply clarsimp
+    prefer 2
+    apply simp
+   apply (clarsimp simp: asids_consistent_def)
+   apply (rule conjI)
+    apply (clarsimp simp: snapshot_update_current'2_def snapshot_update_current2_def)
+    apply (rule conjI)
+     apply (clarsimp simp : \<I>\<C>_def)  
+     apply (drule_tac x = "addr_val v" in spec, simp)
+    apply clarsimp
+    apply (clarsimp simp : \<I>\<C>_def) 
+    apply (drule_tac x = "addr_val v" in spec, simp)
+   apply (case_tac "aa \<noteq> asid s")
+    apply (subgoal_tac "snapshot_update_current'2 (ptable_snapshot s) (incon_set s) (heap s) (root s) (asid s) aa v =
+           (ptable_snapshot s)  aa v")
+     apply (simp only:)
+     apply (drule_tac x = ra in spec)
+     apply (drule_tac x = aa in spec)
+     apply clarsimp
+    apply (clarsimp simp: snapshot_update_current'2_def snapshot_update_current2_def)
+   apply (clarsimp simp: snapshot_update_current'2_def snapshot_update_current2_def)
+   apply (rule)+
+     apply (clarsimp simp : \<I>\<C>_def) 
+     apply (drule_tac x = "addr_val v" in spec, simp)
+    apply clarsimp
+    apply (subgoal_tac "ra =  root s", simp)
+    apply (clarsimp simp: mmu_layout_def)
+    apply (clarsimp simp: ran_def partial_inj_def)
+    apply fastforce
+   apply clarsimp
+   apply (clarsimp simp : \<I>\<C>_def) 
+   apply (drule_tac x = "addr_val v" in spec, simp)
+  apply clarsimp
+  apply (subgoal_tac "incon_load_incon (snapshot_update_current'2 (ptable_snapshot s) (incon_set s) (heap s) (root s) (asid s))
+                      (asid s) (heap s) = {}")
+   prefer 2
+   apply (clarsimp simp: incon_load_incon_def snapshot_update_current'2_def snapshot_update_current2_def)
+   apply (rule)+
+    apply (clarsimp simp : \<I>\<C>_def) 
+    apply (drule_tac x = "addr_val x" in spec, simp)
+   apply (rule)+
+   apply (clarsimp simp : \<I>\<C>_def) 
+   apply (drule_tac x = "addr_val x" in spec, simp)
+  apply simp
+  apply (subgoal_tac "incon_load2
+                      (snapshot_update_current'2
+                        (snapshot_update_current'2 (ptable_snapshot s) (incon_set s) (heap s) (root s) (asid s))
+                        (incon_load_incon (ptable_snapshot s) 0 (heap s) \<union> incon_load2 (ptable_snapshot s) 0 (heap s) (root s) \<union>
+                         ptable_comp 0 (heap s) (heap s) (root s) (Addr r))
+                        (heap s) (Addr r) 0)
+                      (asid s) (heap s) (Addr r) = 
+   incon_load2         (snapshot_update_current'2 (ptable_snapshot s) (incon_set s) (heap s) (root s) (asid s))
+                      (asid s) (heap s) (Addr r)")
 
-
+   prefer 2
+   apply (clarsimp simp: incon_load2_def snapshot_update_current'2_def snapshot_update_current2_def)
+  apply simp
+  apply (subgoal_tac "Addr r = root s")
+   prefer 2
+   apply (clarsimp simp: mmu_layout_def)
+   apply (clarsimp simp: ran_def partial_inj_def)
+   apply fastforce
+  apply simp
+  apply (thin_tac "incon_load2
+           (snapshot_update_current'2 (snapshot_update_current'2 (ptable_snapshot s) (incon_set s) (heap s) (root s) (asid s))
+             (incon_load_incon (ptable_snapshot s) 0 (heap s) \<union> incon_load2 (ptable_snapshot s) 0 (heap s) (root s) \<union> ptable_comp 0 (heap s) (heap s) (root s) (root s)) (heap s) (root s) 0)
+           (asid s) (heap s) (root s) =
+          incon_load2 (snapshot_update_current'2 (ptable_snapshot s) (incon_set s) (heap s) (root s) (asid s)) (asid s) (heap s) (root s)")
+  apply (thin_tac "incon_load_incon (snapshot_update_current'2 (ptable_snapshot s) (incon_set s) (heap s) (root s) (asid s)) (asid s)
+           (heap s) =
+          {}")
+  apply (subgoal_tac "incon_load2 (snapshot_update_current'2 (ptable_snapshot s) (incon_set s) (heap s) (root s) (asid s)) (asid s) (heap s) (root s) =
+                        {}")
+   prefer 2
+   apply (clarsimp simp: asids_consistent_def incon_load2_def snapshot_update_current'2_def 
+      snapshot_update_current2_def)
+  apply simp
+  apply (rule asid_rewrite2)
+    prefer 2
+    apply simp
+   prefer 2 apply simp
+  apply (clarsimp simp: asids_consistent_def)
+  apply (rule conjI)
+   apply (clarsimp simp: snapshot_update_current'2_def snapshot_update_current2_def)
+  apply (case_tac "aa \<noteq> asid s")
+   apply (subgoal_tac "snapshot_update_current'2 (ptable_snapshot s) (incon_set s) (heap s) (root s) (asid s) aa v =
+           (ptable_snapshot s)  aa v")
+    apply (simp only:)
+   apply (drule_tac x = ra in spec)
+   apply (drule_tac x = aa in spec)
+   apply clarsimp
+   apply (clarsimp simp: snapshot_update_current'2_def snapshot_update_current2_def)
+  by (clarsimp simp: snapshot_update_current'2_def snapshot_update_current2_def)
 
 
 end
