Logic/VCG_Check.thy
@@ -10,7 +10,7 @@ begin
 
 
 lemma  write_consistent_defined_address:
-  "\<Turnstile> \<lbrace> \<lambda>s. aval lval s = Some vp \<and> aval rval s = Some v \<and> (asid s, Addr vp) \<notin> incon_set s \<and>
+  "\<Turnstile> \<lbrace> \<lambda>s. aval lval s = Some vp \<and> aval rval s = Some v \<and> Addr vp \<notin> incon_set s \<and>
       ptable_lift_m (heap s) (root s) (mode s) (Addr vp) = Some pp \<rbrace>  lval ::= rval \<lbrace>\<lambda>s. heap s pp = Some v \<rbrace>"
    by vcgm
  
@@ -18,8 +18,8 @@ lemma  write_consistent_defined_address:
 
 
 lemma [simp]:
-  "mem_read_hp' (asid s) (incon_set s) (heap s) (root s) (mode s)(Addr x2) = Some v
-                \<Longrightarrow> mem_read_hp' (asid s) {} (heap s) (root s) (mode s) (Addr x2) = Some v"
+  "mem_read_hp'  (incon_set s) (heap s) (root s) (mode s) (Addr x2) = Some v
+                \<Longrightarrow> mem_read_hp'  {} (heap s) (root s) (mode s) (Addr x2) = Some v"
   by (clarsimp simp: mem_read_hp'_def split: if_split_asm)
 
 
@@ -36,14 +36,17 @@ lemma [simp]:
 
 
 lemma flush_TLB_mem_write:
-  "\<Turnstile> \<lbrace> \<lambda>s. aval lval s = Some vp \<and> aval rval s = Some v \<and> (asid s, Addr vp) \<in> incon_set s \<and>  mode s = Kernel \<and> 
+  "\<Turnstile> \<lbrace> \<lambda>s. aval lval s = Some vp \<and> aval rval s = Some v \<and> Addr vp \<in> incon_set s \<and>  mode s = Kernel \<and> 
       ptable_lift_m (heap s) (root s) (mode s) (Addr vp) = Some pp \<rbrace>  Flush flushTLB ;; lval ::= rval \<lbrace>\<lambda>s. heap s pp = Some v \<rbrace>"
   by vcgm
 
+(*
 lemma[simp]:
-  "mem_read_hp' (asid s) (incon_set s) (heap s) (root s) (mode s) (Addr x2) = Some v
+  "mem_read_hp' (incon_set s) (heap s) (root s) (mode s) (Addr x2) = Some v
                 \<Longrightarrow> mem_read_hp' (asid s) {av \<in> incon_set s. fst av \<noteq> asid s} (heap s) (root s) (mode s) (Addr x2) = Some v"
   by (clarsimp simp: mem_read_hp'_def split: if_split_asm)
+
+
 
 lemma [simp]:
   " incon_set s - ({asid s} \<times> UNIV) = {av \<in> incon_set s. fst av \<noteq> asid s} "
@@ -90,6 +93,6 @@ lemma flush_ASID_va_mem_write:
       ptable_lift_m (heap s) (root s) (mode s) (Addr vp) = Some pp \<rbrace>  Flush (flushASIDvarange a {Addr vp}) ;; lval ::= rval \<lbrace>\<lambda>s. heap s pp = Some v \<rbrace>"
   by vcgm
  
-
+*)
 
 end
